Update IO folder

rupicola/io/ExpRel.fst
@@ -9,12 +9,11 @@ open QTyp
 open IO
 open Trace
 
-type io_cexp (t:qType) =
-  io (get_Type t)
+(** Section 8.1: https://www.cs.uoregon.edu/research/summerschool/summer24/lectures/Ahmed.pdf **)
 
 (** Cross Language Binary Logical Relation between F* and STLC expressions
      for __closed terms__. **)
-let rec (∋) (t:qType) (p:(history * (get_Type t) * closed_exp)) : Tot Type0 (decreases %[get_rel t;0]) =
+let rec (∋) (t:qType) (p:(history * fs_val t * closed_exp)) : Tot Type0 (decreases %[get_rel t;0]) =
   let (h, fs_v, e) = p in
   match get_rel t with // way to "match" on F* types
   | QUnit -> fs_v == () /\ e == EUnit
@@ -24,7 +23,7 @@ let rec (∋) (t:qType) (p:(history * (get_Type t) * closed_exp)) : Tot Type0 (d
     match e with
     | ELam e' ->
       (forall (v:value) (fs_v:t1) (lt_v:local_trace h). pack qt1 ∋ (h++lt_v, fs_v, v) ==>
-        pack qt2 ∶(h++lt_v, fs_f fs_v, subst_beta v e'))
+        pack qt2 ⦂ (h++lt_v, fs_f fs_v, subst_beta v e'))
     | _ -> False
   end
   | QArrIO #t1 #t2 qt1 qt2 -> begin
@@ -32,7 +31,7 @@ let rec (∋) (t:qType) (p:(history * (get_Type t) * closed_exp)) : Tot Type0 (d
     match e with
     | ELam e' -> // instead quantify over h'' - extensions of the history
       (forall (v:value) (fs_v:t1) (lt_v:local_trace h). pack qt1 ∋ (h++lt_v, fs_v, v) ==>
-        pack qt2 ⦂ (h++lt_v, fs_f fs_v, subst_beta v e'))
+        pack qt2 ⪾ (h++lt_v, fs_f fs_v, subst_beta v e'))
     | _ -> False
   end
   | QPair #t1 #t2 qt1 qt2 -> begin
@@ -41,29 +40,34 @@ let rec (∋) (t:qType) (p:(history * (get_Type t) * closed_exp)) : Tot Type0 (d
         pack qt1 ∋ (h, fst #t1 #t2 fs_v, e1) /\ pack qt2 ∋ (h, snd #t1 #t2 fs_v, e2)
     | _ -> False
   end
-                           (** vvvvvvvvvv defined over F* values **)
-and (∶) (t:qType) (p:history * get_Type t * closed_exp) : Tot Type0 (decreases %[get_rel t;1]) =
+  | QSum #t1 #t2 qt1 qt2 -> begin
+    let fs_v : either t1 t2 = fs_v in
+    match fs_v, e with
+    | Inl fs_v', EInl e' -> pack qt1 ∋ (h, fs_v', e')
+    | Inr fs_v', EInr e' -> pack qt2 ∋ (h, fs_v', e')
+    | _ -> False
+  end
+                           (** vvvvvvvvvv defined over values **)
+and (⦂) (t:qType) (p:history * fs_val t * closed_exp) : Tot Type0 (decreases %[get_rel t;1]) =
   let (h, fs_e, e) = p in
   forall (e':closed_exp).
     steps e e' h [] ==> irred e' h ==>
     t ∋ (h, fs_e, e')
-                           (** vvvvvvvvvv defined over IO computations **)
-and (⦂) (t:qType) (p:history * io_cexp t * closed_exp) : Tot Type0 (decreases %[get_rel t;1]) =
+                           (** vvvvvvvvvv defined over producers **)
+and (⪾) (t:qType) (p:history * fs_prod t * closed_exp) : Tot Type0 (decreases %[get_rel t;1]) =
   let (h, fs_e, e) = p in
   forall lt (e':closed_exp).
     steps e e' h lt ==> irred e' (h++lt) ==>
     (exists fs_r. t ∋ (h++lt, fs_r, e') /\ (forall p. theta fs_e h p ==> p lt fs_r))
                            (** TODO: ^^^^^^^^^^^^^^^^^^^^^^^^^^^^^^^^^^ check this **)
 
-(**  forall lt fs_r.
-    (forall p. theta fs_e h p ==> p lt fs_r) ==>
-      (forall (e':closed_exp). steps e e' h lt ==>  t ∋ (h++lt, fs_r, e'))**)
-
-(** Section 8.1: https://www.cs.uoregon.edu/research/summerschool/summer24/lectures/Ahmed.pdf **)
-
 let lem_values_are_expressions t h fs_e e : (** lemma used by Amal **)
   Lemma (requires t ∋ (h, fs_e, e))
-        (ensures  t ⦂ (h, io_return fs_e, e)) = admit ()
+        (ensures  t ⦂ (h, fs_e, e)) = admit ()
+
+let lem_values_are_producers t h fs_e e : (** lemma used by Amal **)
+  Lemma (requires t ∋ (h, fs_e, e))
+        (ensures  t ⪾ (h, io_return fs_e, e)) = admit ()
 
 let rec lem_values_are_values t h fs_e (e:closed_exp) :
   Lemma (requires t ∋ (h, fs_e, e))
@@ -78,6 +82,10 @@ let rec lem_values_are_values t h fs_e (e:closed_exp) :
     let EPair e1 e2 = e in
     lem_values_are_values (pack qt1) h (fst #t1 #t2 fs_e) e1;
     lem_values_are_values (pack qt2) h (snd #t1 #t2 fs_e) e2
+  | QSum #t1 #t2 qt1 qt2 ->
+    match fs_e, e with
+    | Inl fs_e', EInl e' -> lem_values_are_values (pack qt1) h fs_e' e'
+    | Inr fs_e', EInr e' -> lem_values_are_values (pack qt2) h fs_e' e'
 
 (** F* Evaluation Environment : variable -> value **)
 
@@ -102,25 +110,38 @@ let (∽) (#g:typ_env) #b (h:history) (fsG:eval_env g) (s:gsub g b) : Type0 =
 
 (** Cross Language Binary Logical Relation between F* and STLC expressions
      for __open terms__. **)
-let equiv (#g:typ_env) (t:qType) (fs_e:io_oexp g t) (e:exp) : Type0 =
+let equiv_oval (#g:typ_env) (t:qType) (fs_e:fs_oval g t) (e:exp) : Type0 =
   fv_in_env g e /\
   forall b (s:gsub g b) (fsG:eval_env g) (h:history).
     fsG `(∽) h` s ==> t ⦂ (h, fs_e fsG, gsubst s e)
 
-let equiv_closed (#t:qType) (fs_e:io_cexp t) (e:exp) : Type0 =
-  equiv #empty t (fun _ -> fs_e) e
+let equiv_oprod (#g:typ_env) (t:qType) (fs_e:fs_oprod g t) (e:exp) : Type0 =
+  fv_in_env g e /\
+  forall b (s:gsub g b) (fsG:eval_env g) (h:history).
+    fsG `(∽) h` s ==> t ⪾ (h, fs_e fsG, gsubst s e)
 
-let safety (#t:qType) (fs_e:io_cexp t) (e:exp) : Lemma
-  (requires (equiv_closed fs_e e))
+let equiv_val (#t:qType) (fs_e:fs_val t) (e:exp) : Type0 =
+  equiv_oval #empty t (fun _ -> fs_e) e
+
+let equiv_prod (#t:qType) (fs_e:fs_prod t) (e:exp) : Type0 =
+  equiv_oprod #empty t (fun _ -> fs_e) e
+
+let safety_val (#t:qType) (fs_e:fs_val t) (e:exp) : Lemma
+  (requires (equiv_val fs_e e))
+  (ensures (forall h. safe e h)) =
+  admit ()
+
+let safety (#t:qType) (fs_e:fs_prod t) (e:exp) : Lemma
+  (requires (equiv_prod fs_e e))
   (ensures (forall h. safe e h)) =
   introduce forall h (e':closed_exp) (lt:local_trace h).
     steps e e' h lt ==> is_value e' \/ can_step e' (h++lt) with begin
     introduce steps e e' h lt ==> is_value e' \/ can_step e' (h++lt) with _. begin
       introduce irred e' (h++lt) ==> is_value e' with _. begin
         eliminate forall b (s:gsub empty b) (fsG:eval_env empty) (h:history).
-          fsG `(∽) h` s ==> t ⦂ (h, fs_e, gsubst s e)
+          fsG `(∽) h` s ==> t ⪾ (h, fs_e, gsubst s e)
         with  true gsub_empty empty_eval h;
-        assert (t ⦂ (h, fs_e, e));
+        assert (t ⪾ (h, fs_e, e));
         eliminate exists fs_r. t ∋ (h++lt, fs_r, e') /\ (forall p. theta fs_e h p ==> p lt fs_r)
         returns is_value e' with _. begin
           assert (t ∋ (h++lt, fs_r, e'));
@@ -131,76 +152,111 @@ let safety (#t:qType) (fs_e:io_cexp t) (e:exp) : Lemma
     end
   end
 
-let (≈) (#g:typ_env) (#t:qType) (fs_v:io_oexp g t) (e:exp) : Type0 =
-  equiv #g t fs_v e
+let (≈) (#g:typ_env) (#t:qType) (fs_v:fs_oval g t) (e:exp) : Type0 =
+  equiv_oval #g t fs_v e
 
 (** Equiv closed terms **)
-let equiv_closed_terms (#t:qType) (fs_e:io (get_Type t)) (e:closed_exp) :
-  Lemma (requires equiv #empty t (fun _ -> fs_e) e)
-        (ensures  t ⦂ (fs_e, e)) =
-  eliminate forall b (s:gsub empty b) (fsG:eval_env empty).
-    fsG ∽ s ==> t ⦂ ((fun _ -> fs_e) fsG, gsubst s e) with true gsub_empty empty_eval
+let lem_equiv_val (#t:qType) (fs_e:fs_val t) (e:closed_exp) :
+  Lemma (requires equiv_val fs_e e)
+        (ensures forall h. t ⦂ (h, fs_e, e)) =
+  admit ()
 
-let lem_equiv_exp_are_equiv (g:typ_env) (#t:qType) (fs_e:io (get_Type t)) (e:closed_exp) :
-  Lemma (requires t ⦂ (fs_e, e))
-        (ensures  equiv #empty t (fun _ -> fs_e) e) =
-  introduce forall b (s:gsub empty b) (fsG:eval_env empty).
-    fsG ∽ s ==> t ⦂ ((fun _ -> fs_e) fsG, gsubst s e) with begin
-    assert (gsubst s e == e)
+let lem_equiv_val' (#t:qType) (fs_e:fs_val t) (e:closed_exp) :
+  Lemma (requires forall h. t ⦂ (h, fs_e, e))
+        (ensures equiv_val fs_e e) =
+  admit ()
+
+let lem_equiv_prod (#t:qType) (fs_e:fs_prod t) (e:closed_exp) :
+  Lemma (requires equiv_prod fs_e e)
+        (ensures forall h. t ⪾ (h, fs_e, e)) =
+  eliminate forall b (s:gsub empty b) (fsG:eval_env empty). forall h.
+    fsG `(∽) h` s ==> t ⪾ (h, (fun _ -> fs_e) fsG, gsubst s e) with true gsub_empty empty_eval
+
+let lem_equiv_prod' (g:typ_env) (#t:qType) (fs_e:fs_prod t) (e:closed_exp) :
+  Lemma (requires (forall h. t ⪾ (h, fs_e, e)))
+        (ensures equiv_prod fs_e e) =
+  introduce forall b (s:gsub empty b) (fsG:eval_env empty) (h':history).
+    fsG `(∽) h'` s ==> t ⪾ (h', (fun _ -> fs_e) fsG, gsubst s e) with begin
+    introduce fsG `(∽) h'` s ==> t ⪾ (h', (fun _ -> fs_e) fsG, gsubst s e) with _. begin
+      assert (gsubst s e == e);
+      assert ((fun _ -> fs_e) fsG == fs_e);
+      eliminate forall h. t ⪾ (h, fs_e, e) with h'
+    end
   end
 
 (** Rules **)
 
 let equiv_unit g
-  : Lemma ((fun (_:eval_env g) -> io_return ()) `equiv qUnit` EUnit)
+  : Lemma ((fun (_:eval_env g) -> ()) `equiv_oval qUnit` EUnit)
   =
-  introduce forall b (s:gsub g b) fsG. fsG ∽ s ==> qUnit ⦂ (io_return (), gsubst s EUnit) with begin
+  introduce forall b (s:gsub g b) fsG h. fsG `(∽) h` s ==> qUnit ⦂ (h, (), gsubst s EUnit) with begin
     introduce _ ==> _ with _. begin
-      assert (qUnit ∋ ((), EUnit));
-      lem_values_are_expressions qUnit () EUnit
+      assert (qUnit ∋ (h, (), EUnit));
+      lem_values_are_expressions qUnit h () EUnit
     end
   end
 
 let equiv_true g
-  : Lemma ((fun (_:eval_env g) -> io_return true) `equiv qBool` ETrue)
+  : Lemma ((fun (_:eval_env g) -> true) `equiv_oval qBool` ETrue)
   =
-  introduce forall b (s:gsub g b) fsG. fsG ∽ s ==> qBool ⦂ (io_return true, gsubst s ETrue) with begin
+  introduce forall b (s:gsub g b) fsG h. fsG `(∽) h` s ==> qBool ⦂ (h, true, gsubst s ETrue) with begin
     introduce _ ==> _ with _. begin
-      assert (qBool ∋ (true, ETrue));
-      lem_values_are_expressions qBool true ETrue
+      assert (qBool ∋ (h, true, ETrue));
+      lem_values_are_expressions qBool h true ETrue
     end
   end
 
 let equiv_false g
-  : Lemma ((fun (_:eval_env g) -> io_return false) `equiv qBool` EFalse)
+  : Lemma ((fun (_:eval_env g) -> false) `equiv_oval qBool` EFalse)
   =
-  introduce forall b (s:gsub g b) fsG. fsG ∽ s ==> qBool ⦂ (io_return false, gsubst s EFalse) with begin
+  introduce forall b (s:gsub g b) fsG h. fsG `(∽) h` s ==> qBool ⦂ (h, false, gsubst s EFalse) with begin
     introduce _ ==> _ with _. begin
-      assert (qBool ∋ (false, EFalse));
-      lem_values_are_expressions qBool false EFalse
+      assert (qBool ∋ (h, false, EFalse));
+      lem_values_are_expressions qBool h false EFalse
     end
   end
 
 let equiv_var g (x:var{Some? (g x)})
-  : Lemma ((fun (fsG:eval_env g) -> io_return (index fsG x)) ≈ EVar x)
+  : Lemma ((fun (fsG:eval_env g) -> index fsG x) ≈ EVar x)
   =
-  introduce forall b (s:gsub g b) fsG. fsG ∽ s ==> Some?.v (g x) ⦂ (io_return (index fsG x), gsubst s (EVar x)) with begin
+  introduce forall b (s:gsub g b) fsG h. fsG `(∽) h` s ==> Some?.v (g x) ⦂ (h, index fsG x, gsubst s (EVar x)) with begin
     introduce _ ==> _ with _. begin
-      assert (Some?.v (g x) ∋ (index fsG x, s x));
-      lem_values_are_expressions (Some?.v (g x)) (index fsG x) (s x)
+      assert (Some?.v (g x) ∋ (h, index fsG x, s x));
+      lem_values_are_expressions (Some?.v (g x)) h (index fsG x) (s x)
     end
   end
 
-let equiv_lam #g (t1:qType) (t2:qType) (f:fs_oexp g (t1 ^-> t2)) (body:exp) : Lemma
-  (requires (fun (fsG:eval_env (extend t1 g)) -> io_bind (f (tail #t1 fsG)) (fun f -> f (hd fsG))) ≈ body)
-  (ensures f ≈ (ELam body)) = admit ()
-  (*lem_fv_in_env_lam g t1 body;
+(** Used in compilation **)
+let equiv_var0 (g:typ_env) (t:qType)
+  : Lemma ((fun (fsG:eval_env (extend t g)) -> hd fsG) ≈ EVar 0)
+  =
+  introduce forall b (s:gsub (extend t g) b) fsG h. fsG `(∽) h` s ==>  t ⦂ (h, hd fsG, gsubst s (EVar 0)) with begin
+    introduce _ ==> _ with _. begin
+      index_0_hd fsG;
+      assert (t ∋ (h, hd fsG, s 0));
+      lem_values_are_expressions t h (hd fsG) (s 0)
+    end
+  end
+
+(** Used in compilation **)
+let equiv_varS (#g:typ_env) #a #t (s:fs_oval g a) (e:exp)
+  : Lemma
+      (requires (equiv_oval #g a s e))
+      (ensures (equiv_oval #(extend t g) a (fun fsG -> s (tail fsG)) (subst sub_inc e)))
+  = admit ()
+
+let equiv_lam #g (#t1:qType) (#t2:qType) (fs_body:fs_oval (extend t1 g) t2) (body:exp) : Lemma
+  (requires fs_body ≈ body)
+  (ensures (fun fsG x -> fs_body (stack fsG x)) `equiv_oval (t1 ^-> t2)` (ELam body)) =
+  admit () (**
+  lem_fv_in_env_lam g t1 body;
   let g' = extend t1 g in
-  introduce forall b (s:gsub g b) fsG. fsG ∽ s ==> (t1 ^-> t2) ⦂ (f fsG, gsubst s (ELam body)) with begin
+  let f : fs_oval g (t1 ^-> t2) = fun fsG x -> fs_body (stack fsG x) in
+  introduce forall b (s:gsub g b) fsG. fsG ∽ s ==>  (t1 ^-> t2) ⦂ (f fsG, gsubst s (ELam body)) with begin
     introduce _ ==> _ with _. begin
       let body' = subst (sub_elam s) body in
       assert (gsubst s (ELam body) == ELam body');
-      introduce forall (v:value) (fs_v:get_Type t1). t1 ∋ (fs_v, v) ==>  t2 ⦂ (f fsG fs_v, subst_beta v body') with begin
+      introduce forall (v:value) (fs_v:fs_val t1). t1 ∋ (fs_v, v) ==>  t2 ⦂ (f fsG fs_v, subst_beta v body') with begin
         introduce _ ==> _ with _. begin
           let s' = gsub_extend s t1 v in
           let fsG' = stack fsG fs_v in
@@ -220,20 +276,19 @@ let equiv_lam #g (t1:qType) (t2:qType) (f:fs_oexp g (t1 ^-> t2)) (body:exp) : Le
       lem_values_are_expressions (t1 ^-> t2) (f fsG) (gsubst s (ELam body));
       assert ((t1 ^-> t2) ⦂ (f fsG, gsubst s (ELam body)))
     end
-  end*)
+  end**)
 
+
+#push-options "--z3rlimit 5000 --fuel 5000"
 let equiv_app #g
   (#t1:qType) (#t2:qType)
-  (fs_e1:fs_oexp g (t1 ^-> t2)) (fs_e2:fs_oexp g t1)
+  (fs_e1:fs_oval g (t1 ^-> t2)) (fs_e2:fs_oval g t1)
   (e1:exp) (e2:exp)
   : Lemma
     (requires fs_e1 ≈ e1 /\ fs_e2 ≈ e2)
-    (ensures
-        (fun fsG -> io_bind (fs_e1 fsG) (fun f -> io_bind (fs_e2 fsG) f))
-        ≈
-        (EApp e1 e2))
-  = admit ()
-  (**
+    (ensures (fun fsG -> (fs_e1 fsG) (fs_e2 fsG)) ≈ (EApp e1 e2))
+  =
+  admit () (**
   lem_fv_in_env_app g e1 e2;
   introduce forall b (s:gsub g b) fsG. fsG ∽ s ==> t2 ⦂ ((fs_e1 fsG) (fs_e2 fsG), gsubst s (EApp e1 e2)) with begin
     let fs_e1 = fs_e1 fsG in
@@ -257,7 +312,7 @@ let equiv_app #g
               assert (steps e2 e2');
               assert (irred e2')
             end;
-            eliminate forall (v:value) (fs_v:get_Type t1). t1 ∋ (fs_v, v) ==>
+            eliminate forall (v:value) (fs_v:fs_val t1). t1 ∋ (fs_v, v) ==>
               t2 ⦂ (fs_e1 fs_v, subst_beta v e11)
             with e2' fs_e2;
             assert (t2 ⦂ (fs_e, subst_beta e2' e11));
@@ -266,20 +321,16 @@ let equiv_app #g
         end
       end
     end
-  end **)
+  end**)
 
-let equiv_if #g (#t:qType) (fs_e1:fs_oexp g qBool) (fs_e2:fs_oexp g t) (fs_e3:fs_oexp g t) (e1:exp) (e2:exp) (e3:exp) : Lemma
+let equiv_if #g (#t:qType) (fs_e1:fs_oval g qBool) (fs_e2:fs_oval g t) (fs_e3:fs_oval g t) (e1:exp) (e2:exp) (e3:exp) : Lemma
   (requires fs_e1 ≈ e1 /\ fs_e2 ≈ e2 /\ fs_e3 ≈ e3)
-  (ensures (
-    (fun fsG ->
-      io_bind (fs_e1 fsG) (fun b -> if b then fs_e2 fsG else fs_e3 fsG))
-    ≈
-    (EIf e1 e2 e3))) =
+  (ensures (fun fsG -> if fs_e1 fsG then fs_e2 fsG else fs_e3 fsG) ≈ EIf e1 e2 e3) =
   admit ()
   (**
   lem_fv_in_env_if g e1 e2 e3;
   introduce forall b (s:gsub g b) fsG. fsG ∽ s ==> t ⦂ ((if fs_e1 fsG then fs_e2 fsG else fs_e3 fsG), gsubst s (EIf e1 e2 e3)) with begin
-    (*let fs_e1 = fs_e1 fsG in
+    let fs_e1 = fs_e1 fsG in
     let fs_e = if fs_e1 then fs_e2 fsG else fs_e3 fsG in
     let e = EIf (gsubst s e1) (gsubst s e2) (gsubst s e3) in
     assert (gsubst s (EIf e1 e2 e3) == e);
@@ -300,25 +351,25 @@ let equiv_if #g (#t:qType) (fs_e1:fs_oexp g qBool) (fs_e2:fs_oexp g t) (fs_e3:fs
           )
         end
       end
-    end*)
-    admit ()
-  end
-  **)
+    end
+  end**)
+#pop-options
 
-(**
-let equiv_pair #g (#t1 #t2:qType) (fs_e1:fs_oexp g t1) (fs_e2:fs_oexp g t2) (e1:exp) (e2:exp) : Lemma
+let equiv_pair #g (#t1 #t2:qType) (fs_e1:fs_oval g t1) (fs_e2:fs_oval g t2) (e1:exp) (e2:exp) : Lemma
   (requires fs_e1 ≈ e1 /\ fs_e2 ≈ e2)
-  (ensures equiv #g (t1 ^* t2) (fun fsG -> io_return (fs_e1 fsG, fs_e2 fsG)) (EPair e1 e2)) =
+  (ensures (fun fsG -> (fs_e1 fsG, fs_e2 fsG)) `equiv_oval (t1 ^* t2)` EPair e1 e2) =
+  admit ()
+  (**
   lem_fv_in_env_pair g e1 e2;
   let t = t1 ^* t2 in
-  introduce forall b (s:gsub g b) fsG. fsG ∽ s ==>  t ⦂ (io_return (fs_e1 fsG, fs_e2 fsG), gsubst s (EPair e1 e2)) with begin
+  introduce forall b (s:gsub g b) fsG. fsG ∽ s ==>  t ⦂ ((fs_e1 fsG, fs_e2 fsG), gsubst s (EPair e1 e2)) with begin
     let fs_e1 = fs_e1 fsG in
     let fs_e2 = fs_e2 fsG in
     let fs_e = (fs_e1, fs_e2) in
     let e = EPair (gsubst s e1) (gsubst s e2) in
     assert (gsubst s (EPair e1 e2) == e);
     let EPair e1 e2 = e in
-    introduce fsG ∽ s ==>  t ⦂ (io_return fs_e, e) with _. begin
+    introduce fsG ∽ s ==>  t ⦂ (fs_e, e) with _. begin
       introduce forall (e':closed_exp). steps e e' /\ irred e' ==> t ∋ (fs_e, e') with begin
         introduce _ ==> t ∋ (fs_e, e') with h. begin
           let steps_e_e' : squash (steps e e') = () in
@@ -334,11 +385,13 @@ let equiv_pair #g (#t1 #t2:qType) (fs_e1:fs_oexp g t1) (fs_e2:fs_oexp g t2) (e1:
         end
       end
     end
-  end
+  end **)
 
-let equiv_pair_fst_app #g (#t1 #t2:qType) (fs_e12:fs_oexp g (t1 ^* t2)) (e12:exp) : Lemma
-  (requires equiv #g (t1 ^* t2) fs_e12 e12) (** is this too strict? we only care for the left to be equivalent. **)
-  (ensures equiv #g t1 (fun fsG -> fst (fs_e12 fsG)) (EFst e12)) =
+let equiv_pair_fst_app #g (#t1 #t2:qType) (fs_e12:fs_oval g (t1 ^* t2)) (e12:exp) : Lemma
+  (requires fs_e12 `equiv_oval (t1 ^* t2)` e12) (** is this too strict? we only care for the left to be equivalent. **)
+  (ensures (fun fsG -> fst (fs_e12 fsG)) `equiv_oval t1` (EFst e12)) =
+  admit ()
+  (**
   introduce forall b (s:gsub g b) fsG. fsG ∽ s ==>  t1 ⦂ (fst (fs_e12 fsG), gsubst s (EFst e12)) with begin
     let fs_e12 = fs_e12 fsG in
     let fs_e = fst fs_e12 in
@@ -350,7 +403,10 @@ let equiv_pair_fst_app #g (#t1 #t2:qType) (fs_e12:fs_oexp g (t1 ^* t2)) (e12:exp
         introduce _ ==> t1 ∋ (fs_e, e') with h. begin
           let steps_e_e' : squash (steps e e') = () in
           FStar.Squash.map_squash #_ #(squash (t1 ∋ (fs_e, e'))) steps_e_e' (fun steps_e_e' ->
-            let e12' = destruct_steps_epair_fst e12 e' steps_e_e' in
+            safety (t1 ^* t2) fs_e12 e12;
+            let t1_typ = type_quotation_to_typ (get_rel t1) in
+            let t2_typ = type_quotation_to_typ (get_rel t2) in
+            let e12' = destruct_steps_epair_fst e12 e' steps_e_e' t1_typ t2_typ in
             eliminate (t1 ^* t2) ⦂ (fs_e12, e12) /\ steps e12 e12' /\ irred e12'
             returns (t1 ^* t2) ∋ (fs_e12, e12') with _ _. ();
             let EPair e1' e2' = e12' in
@@ -362,48 +418,15 @@ let equiv_pair_fst_app #g (#t1 #t2:qType) (fs_e12:fs_oexp g (t1 ^* t2)) (e12:exp
       end
     end
   end
+**)
 
-let equiv_pair_fst g (t1 t2:qType)
+let equiv_pair_snd_app #g (#t1 #t2:qType) (fs_e12:fs_oval g (t1 ^* t2)) (e12:exp)
   : Lemma
-    (requires True)
-    (ensures equiv #g ((t1 ^* t2) ^-> t1) (fun _ -> fst #(get_Type t1) #(get_Type t2)) (ELam (EFst (EVar 0))))
+    (requires fs_e12 `equiv_oval (t1 ^* t2)` e12) (** is this too strict? we only care for the left to be equivalent. **)
+    (ensures (fun fsG -> snd (fs_e12 fsG)) `equiv_oval t2` (ESnd e12))
   =
-  let tp = t1 ^* t2 in
-  let t = tp ^-> t1 in
-  let fs_e : (get_Type t1 & get_Type t2) -> get_Type t1 = fst in
-  let fs_e' : eval_env g -> get_Type t = (fun _ -> fs_e) in
-  let e = ELam (EFst (EVar 0)) in
-  introduce forall b (s:gsub g b) fsG. fsG ∽ s ==>  t ⦂ (fs_e' fsG, gsubst s e) with begin
-    assert (gsubst s e == e);
-    assert (fs_e' fsG == fs_e);
-
-    eliminate True /\ True
-    returns t ∋ (fs_e, e) with _ _. begin
-      introduce forall (v:value) (fs_v:get_Type tp). tp ∋ (fs_v, v) ==>
-        t1 ⦂ (fs_e fs_v, subst_beta v (EFst (EVar 0))) with begin
-        introduce _ ==> _ with _. begin
-          lem_values_are_expressions tp fs_v v;
-          lem_equiv_exp_are_equiv empty #tp fs_v v;
-          assert ((fun _ -> fs_v) `equiv #empty tp` v);
-          equiv_pair_fst_app #empty #t1 #t2 (fun _ -> fs_v) v;
-          assert ((fun _ -> fs_e fs_v) `equiv #empty t1` (EFst v));
-          equiv_closed_terms #t1 (fs_e fs_v) (EFst v);
-          assert (subst_beta v (EFst (EVar 0)) == EFst v);
-          ()
-        end
-      end
-    end;
-
-    assert (t ∋ (fs_e, e));
-    lem_values_are_expressions t fs_e e;
-    assert (t ⦂ (fs_e, e))
-  end
-
-let equiv_pair_snd_app #g (#t1 #t2:qType) (fs_e12:fs_oexp g (t1 ^* t2)) (e12:exp)
-  : Lemma
-    (requires equiv #g (t1 ^* t2) fs_e12 e12) (** is this too strict? we only care for the left to be equivalent. **)
-    (ensures equiv #g t2 (fun fsG -> snd (fs_e12 fsG)) (ESnd e12))
-  =
+  admit ()
+  (**
   introduce forall b (s:gsub g b) fsG. fsG ∽ s ==>  t2 ⦂ (snd (fs_e12 fsG), gsubst s (ESnd e12)) with begin
     let fs_e12 = fs_e12 fsG in
     let fs_e = snd fs_e12 in
@@ -415,7 +438,10 @@ let equiv_pair_snd_app #g (#t1 #t2:qType) (fs_e12:fs_oexp g (t1 ^* t2)) (e12:exp
         introduce _ ==> t2 ∋ (fs_e, e') with h. begin
           let steps_e_e' : squash (steps e e') = () in
           FStar.Squash.map_squash #_ #(squash (t2 ∋ (fs_e, e'))) steps_e_e' (fun steps_e_e' ->
-            let e12' = destruct_steps_epair_snd e12 e' steps_e_e' in
+            safety (t1 ^* t2) fs_e12 e12;
+            let t1_typ = type_quotation_to_typ (get_rel t1) in
+            let t2_typ = type_quotation_to_typ (get_rel t2) in
+            let e12' = destruct_steps_epair_snd e12 e' steps_e_e' t1_typ t2_typ in
             eliminate (t1 ^* t2) ⦂ (fs_e12, e12) /\ steps e12 e12' /\ irred e12'
             returns (t1 ^* t2) ∋ (fs_e12, e12') with _ _. ();
             let EPair e1' e2' = e12' in
@@ -427,40 +453,26 @@ let equiv_pair_snd_app #g (#t1 #t2:qType) (fs_e12:fs_oexp g (t1 ^* t2)) (e12:exp
       end
     end
   end
+  **)
 
-let equiv_pair_snd g (t1 t2:qType)
+let equiv_inl #g (#t1 t2:qType) (fs_e:fs_oval g t1) (e:exp) : Lemma
+  (requires fs_e ≈ e)
+  (ensures (fun fsG -> Inl (fs_e fsG)) `equiv_oval (t1 ^+ t2)` (EInl e)) =
+  admit ()
+
+let equiv_inr #g (t1 #t2:qType) (fs_e:fs_oval g t2) (e:exp) : Lemma
+  (requires fs_e ≈ e)
+  (ensures (fun fsG -> Inr (fs_e fsG)) `equiv_oval (t1 ^+ t2)` (EInr e)) =
+  admit ()
+
+let equiv_case
+  #g
+  (#t1 #t2 #t3:qType)
+  (fs_case:fs_oval g (t1 ^+ t2))
+  (fs_lc:fs_oval (extend t1 g) t3)
+  (fs_rc:fs_oval (extend t2 g) t3)
+  (e_case e_lc e_rc:exp)
   : Lemma
-    (requires True)
-    (ensures equiv #g ((t1 ^* t2) ^-> t2) (fun _ -> snd #(get_Type t1) #(get_Type t2)) (ELam (ESnd (EVar 0))))
-  =
-  let tp = t1 ^* t2 in
-  let t = tp ^-> t2 in
-  let fs_e : (get_Type t1 & get_Type t2) -> get_Type t2 = snd in
-  let fs_e' : eval_env g -> get_Type t = (fun _ -> fs_e) in
-  let e = ELam (ESnd (EVar 0)) in
-  introduce forall b (s:gsub g b) fsG. fsG ∽ s ==>  t ⦂ (fs_e' fsG, gsubst s e) with begin
-    assert (gsubst s e == e);
-    assert (fs_e' fsG == fs_e);
-
-    eliminate True /\ True
-    returns t ∋ (fs_e, e) with _ _. begin
-      introduce forall (v:value) (fs_v:get_Type tp). tp ∋ (fs_v, v) ==>
-        t2 ⦂ (fs_e fs_v, subst_beta v (ESnd (EVar 0))) with begin
-        introduce _ ==> _ with _. begin
-          lem_values_are_expressions tp fs_v v;
-          lem_equiv_exp_are_equiv empty #tp fs_v v;
-          assert ((fun _ -> fs_v) `equiv #empty tp` v);
-          equiv_pair_snd_app #empty #t1 #t2 (fun _ -> fs_v) v;
-          assert ((fun _ -> fs_e fs_v) `equiv #empty t2` (ESnd v));
-          equiv_closed_terms #t2 (fs_e fs_v) (ESnd v);
-          assert (subst_beta v (ESnd (EVar 0)) == ESnd v);
-          ()
-        end
-      end
-    end;
-
-    assert (t ∋ (fs_e, e));
-    lem_values_are_expressions t fs_e e;
-    assert (t ⦂ (fs_e, e))
-  end
-**)
+    (requires fs_case ≈ e_case /\ fs_lc ≈ e_lc /\ fs_rc ≈ e_rc)
+    (ensures (fun fsG -> match fs_case fsG with | Inl x -> fs_lc (stack fsG x) | Inr x -> fs_rc (stack fsG x)) `equiv_oval t3` (ECase e_case e_lc e_rc))
+  = admit ()
